preservation tools on set-based semantics

Logic/Modal/Standard/Kripke/Preservation.lean
@@ -15,8 +15,8 @@ section Generation
 
 class GeneratedSubframe (F F' : Kripke.Frame α) where
   subset : F'.World ⊆ F.World
-  -- rel : ∀ x y : F'.World, F'.Rel' x y → F.Rel' x y
-  closed : ∀ x y : F.World, x ≺ y → y.1 ∈ F'.World
+  rel : ∀ x y : F'.World, F'.Rel' x y ↔ F.Rel' ⟨x, (by aesop)⟩ ⟨y, (by aesop)⟩ -- MEMO: i.e. F.Rel' = F.Rel' ∪ (F.World × F.World)
+  closed : ∀ x : F'.World, ∀ y : F.World, F.Rel' ⟨x.1, (by aesop)⟩ y → y.1 ∈ F'.World
 
 
 end Generation
@@ -35,9 +35,10 @@ protected class Model.reduction {M₁ M₂ : Kripke.Model α β} (f : M₁.World
 
 open Formula
 
-variable {F₁ F₂ : Kripke.Frame α} {M₁ M₂ : Kripke.Model α β}
+variable {F₁ F₂ : Kripke.Frame' α β} {M₁ M₂ : Kripke.Model α β} {p : Formula β}
 
-lemma iff_formula_satisfies_morphism (f : M₁.World → M₂.World) [Model.reduction f] {w : M₁.World} : (M₁, w) ⊧ p ↔ (M₂, (f w)) ⊧ p := by
+lemma iff_formula_satisfies_morphism (f : M₁.World → M₂.World) [Model.reduction f] {w : M₁.World}
+  : (⟨M₁, w⟩ : (M : Model α β) × M.World) ⊧ p ↔ (⟨M₂, (f w)⟩ : (M : Model α β) × M.World) ⊧ p := by
   induction p using Formula.rec' generalizing w with
   | hatom p =>
     constructor;
@@ -52,28 +53,53 @@ lemma iff_formula_satisfies_morphism (f : M₁.World → M₂.World) [Model.redu
       assumption;
     . intro h w' hww';
       exact ih.mpr $ h $ Frame.reduction.forth hww';
-  | _ => simp_all;
+  | _ => simp_all [kripke_satisfies];
 
-lemma iff_formula_valid_on_frame_surjective_morphism (f : F₁ → F₂) [Frame.reduction f] (f_surjective : f.Surjective) : F₁ ⊧ p → F₂ ⊧ p := by
+lemma iff_formula_valid_on_frame_surjective_morphism (f : F₁.World → F₂.World) [Frame.reduction f] (f_surjective : f.Surjective) : F₁ ⊧ p → F₂ ⊧ p := by
   contrapose;
   intro h;
-  obtain ⟨V₂, w₂, h⟩ := by simpa [valid_on_KripkeFrame, valid_on_KripkeModel] using h;
+  obtain ⟨V₂, w₂, hw₂, h⟩ := by simpa [valid_on_KripkeFrame, valid_on_KripkeModel] using h;
   simp [valid_on_KripkeFrame, valid_on_KripkeModel];
 
-  obtain ⟨w₁, e⟩ : ∃ w₁, f w₁ = w₂ := by apply f_surjective;
-  subst e;
+  obtain ⟨w₁, e⟩ := f_surjective ⟨w₂, hw₂⟩; rw [←e] at h;
   let V₁ := λ w a => V₂ (f w) a;
-  use V₁, w₁;
+  use V₁, w₁.1, w₁.2;
 
-  let M₁ : Model α := { Frame := F₁, Valuation := V₁ };
-  let M₂ : Model α := { Frame := F₂, Valuation := V₂ };
+  let M₁ : Model α β := { Frame := F₁, Valuation := V₁ };
+  let M₂ : Model α β := { Frame := F₂, Valuation := V₂ };
   have : Model.reduction (M₁ := M₁) (M₂ := M₂) f := { atomic := by simp_all };
   exact iff_formula_satisfies_morphism (M₁ := M₁) (M₂ := M₂) f |>.not.mpr h;
 
-lemma iff_theory_valid_on_frame_surjective_morphism (f : F₁ → F₂) [Frame.reduction f] (f_surjective : f.Surjective) : F₁ ⊧* T → F₂ ⊧* T := by
+lemma iff_theory_valid_on_frame_surjective_morphism (f : F₁.World → F₂.World) [Frame.reduction f] (f_surjective : f.Surjective) : F₁ ⊧* T → F₂ ⊧* T := by
   simp only [Semantics.realizeSet_iff];
   intro h p hp;
   exact iff_formula_valid_on_frame_surjective_morphism f f_surjective (h hp);
+
+abbrev IrreflexiveFrameClass : FrameClass := λ _ F => Irreflexive F.Rel'
+
+theorem undefinable_irreflexive : ¬∃ (Ax : AxiomSet β), Ax.DefinesKripkeFrameClass IrreflexiveFrameClass := by
+  by_contra hC;
+  obtain ⟨Ax, h⟩ := hC;
+
+  -- MEMO: `Rel := { (x, y) | x ≠ y }`で行けてほしいのだがなぜか通らない．
+  let F₁ : Frame' (Fin 2) β := { World := {0, 1}, Rel := {(⟨0, by simp⟩, ⟨1, by simp⟩), (⟨1, by simp⟩, ⟨0, by simp⟩)} };
+  have hIF₁ : Irreflexive F₁.Rel' := by simp [Irreflexive, Frame.Rel'];
+
+  let F₂ : Frame' (Fin 2) β := { World := {0}, Rel := { (x, y) | x = y } };
+  have hIF₂ : ¬Irreflexive F₂.Rel' := by simp [Irreflexive]; use ⟨0, (by simp)⟩; simp [Frame.Rel'];
+
+  let f : F₁.World → F₂.World := λ _ => ⟨0, (by simp)⟩;
+  have hSur : Function.Surjective f := by simp [Function.Surjective]; aesop;
+  have : Frame.reduction f := {
+    forth := by simp [Frame.Rel'];
+    back := by
+      intro x y Rxy; simp [Frame.Rel'] at Rxy;
+      match x with
+      | ⟨0, _⟩ => use ⟨1, (by simp)⟩; simp_all [Frame.Rel'];
+      | ⟨1, _⟩ => use ⟨0, (by simp)⟩; simp_all [Frame.Rel'];
+  };
+  have : Irreflexive F₂.Rel' := h.mp $ iff_theory_valid_on_frame_surjective_morphism f hSur $ h.mpr hIF₁;
+  contradiction;
 
 end Reduction
 
