Logic/Modal/Standard/Kripke/Kripke.lean
@@ -1,6 +1,6 @@
-import Logic.Modal.Standard.Kripke.Morphism
 import Logic.Modal.Standard.Kripke.Soundness
 import Logic.Modal.Standard.Kripke.Completeness
+import Logic.Modal.Standard.Kripke.Preservation
 
 import Logic.Modal.Standard.Kripke.Geach
 import Logic.Modal.Standard.Kripke.Ver
