Logic/Modal/Standard/Kripke/Reducible.lean
@@ -11,7 +11,7 @@ open Formula
 
 variable
   {α : Type*} [DecidableEq α]
-  {Ax₁ Ax₂ : AxiomSet α} (𝔽₁ 𝔽₂ : FrameClass α)
+  {Ax₁ Ax₂ : AxiomSet α} (𝔽₁ 𝔽₂ : FrameClass' α)
   [sound₁ : Sound Ax₁ᴺ 𝔽₁] [sound₂ : Sound Ax₂ᴺ 𝔽₂]
   [complete₁ : Complete (Ax₁ᴺ) 𝔽₁] [complete₂ : Complete (Ax₂ᴺ) 𝔽₂]
 
@@ -19,8 +19,8 @@ lemma reducible_of_subset_FrameClass (h𝔽 : 𝔽₂ ⊆ 𝔽₁) : Ax₁ᴺ �
   apply System.reducible_iff.mpr;
   intro p hp;
   apply complete₂.complete;
-  intro F hF;
-  exact sound₁.sound hp F $ h𝔽 hF;
+  intro _ F hF;
+  exact sound₁.sound hp F $ h𝔽 _ hF;
 
 /-
 lemma strictreducible_of_ssubset_FrameClass (hne : Ax₂.Nonempty) (h𝔽 : 𝔽₂ ⊂ 𝔽₁) : Ax₁ᴺ <ₛ Ax₂ᴺ := by
